Implement Call in Computation.v

Computation.v
@@ -10,9 +10,13 @@ Reserved Notation "'call' f [[ x ]]" (at level 35).
 Delimit Scope comp_scope with comp.
 Delimit Scope long_comp_scope with long_comp.
 
+Class Context :=
+  { names : Type;
+    dom : names -> Type;
+    cod : names -> Type }.
+
 Section Comp.
-  Variable names : Type.
-  Variables dom cod : names -> Type.
+  Context {ctx : Context}.
 
   Inductive Comp : Type -> Type :=
   | Return : forall A, A -> Comp A
@@ -22,10 +26,10 @@ Section Comp.
 End Comp.
 
 Bind Scope comp_scope with Comp.
-Arguments Bind [_%type _ _ A%type B%type] _%comp _.
-Arguments Call [_%type _ _] name _%comp.
-Arguments Return [_ _ _ _] _.
-Arguments Pick [_ _ _ _] _.
+Arguments Bind {_} [A%type B%type] _%comp _.
+Arguments Call {_} name _%comp.
+Arguments Return {_} [_] _.
+Arguments Pick {_} [_] _.
 
 (*Notation "x >>= y" := (Bind x%comp y%comp) : comp_scope.
 Notation "x <- y ; z" := (Bind y%comp (fun x => z%comp)) : comp_scope.
@@ -41,33 +45,36 @@ Notation "x <- y ; z" := (Bind y%comp (fun x => z%comp))
 Notation "x ;; z" := (Bind x%comp (fun _ => z%comp))
                        (at level 81, right associativity,
                         format "'[v' x ;; '/' z ']'") : comp_scope.
-Notation "{ x  |  P }" := (@Pick _ _ _ _ (fun x => P)) : comp_scope.
-Notation "{ x : A  |  P }" := (@Pick _ _ _ A%type (fun x => P)) : comp_scope.
-Notation "'call' f [[ x ]]" := (@Call _ _ _ f x) : comp_scope.
+Notation "{ x  |  P }" := (@Pick _ _ (fun x => P)) : comp_scope.
+Notation "{ x : A  |  P }" := (@Pick _ A%type (fun x => P)) : comp_scope.
+Notation "'call' f [[ x ]]" := (@Call _ f x) : comp_scope.
+
+Class LookupContext :=
+  { LContext :> Context;
+    lookup : forall name, dom name -> Comp (cod name) }.
+
+Coercion LContext : LookupContext >-> Context.
 
 Record BundledComp A :=
-  Bundle { CompNames : _;
-           CompDom : _;
-           CompCod : _;
-           Unbundle :> @Comp CompNames CompDom CompCod A;
-           Lookup : forall name, CompDom name -> @Comp CompNames CompDom CompCod (CompCod name)}.
+  Bundle { CompContext : LookupContext;
+           Unbundle :> Comp A }.
 
 Delimit Scope bundled_comp_scope with bundled_comp.
 Bind Scope bundled_comp_scope with BundledComp.
 Open Scope bundled_comp_scope.
 
-Notation "``[ c 'with' l ]``" := (@Bundle _ _ _ _ c l) (only parsing) : bundled_comp_scope.
+Notation "``[ c 'with' l ]``" := (@Bundle _ l c) (only parsing) : bundled_comp_scope.
 Notation "`[ c ]`" := ``[ c with _ ]`` : bundled_comp_scope.
-Notation "``[ c 'with' l ]``" := (@Bundle _ _ _ _ c l) : long_comp_scope.
+Notation "``[ c 'with' l ]``" := (``[ c with l ]``)%bundled_comp : long_comp_scope.
 
 Section comp.
-  Definition Lift names dom cod A B (f : A -> B)
-  : @Comp names dom cod A -> @Comp names dom cod B
+  Definition Lift `{ctx : Context} A B (f : A -> B)
+  : Comp A -> Comp B
     := fun x => (x' <- x;
                  Return (f x'))%comp.
 
-  Definition Or names dom cod
-  : @Comp names dom cod bool -> Comp _ _ bool -> Comp _ _ bool
+  Definition Or `{ctx : Context}
+  : Comp bool -> Comp bool -> Comp bool
     := fun c1 c2 =>
          (b1 <- c1;
           if b1
@@ -75,12 +82,10 @@ Section comp.
           else c2)%comp.
 
   Section computes_to.
-    Variable names : Type.
-    Variables dom cod : names -> Type.
-    Variable lookup : forall name, dom name -> @Comp names dom cod (cod name).
+    Context `{ctx : LookupContext}.
 
     (** TODO(JasonGross): Should this be [CoInductive]? *)
-    Inductive computes_to : forall A, @Comp names dom cod A -> A -> Prop :=
+    Inductive computes_to : forall A, Comp A -> A -> Prop :=
     | ReturnComputes : forall A v, @computes_to A (Return v) v
     | BindComputes : forall A B comp_a f comp_a_value comp_b_value,
                        @computes_to A comp_a comp_a_value
@@ -89,11 +94,11 @@ Section comp.
     | PickComputes : forall A (P : Ensemble A) v, P v -> @computes_to A (Pick P) v
     | CallComputes : forall f x x_value fx_value,
                        @computes_to (dom f) x x_value
-                       -> @computes_to (cod f) (@lookup f x_value) fx_value
+                       -> @computes_to (cod f) (@lookup _ f x_value) fx_value
                        -> @computes_to _ (Call f x) fx_value.
 
-    Theorem computes_to_inv A (c : @Comp names dom cod A) v
-    : computes_to c v -> match c in (@Comp _ _ _ A) return A -> Prop with
+    Theorem computes_to_inv A (c : Comp A) v
+    : computes_to c v -> match c in (Comp A) return A -> Prop with
                            | Return _ x => @eq _ x
                            | Bind _ _ x f => fun v => exists comp_a_value,
                                                         computes_to x comp_a_value
@@ -102,7 +107,7 @@ Section comp.
                            | Call f x => fun fx_v =>
                                            exists xv,
                                              computes_to x xv
-                                             /\ computes_to (@lookup f xv) fx_v
+                                             /\ computes_to (@lookup _ f xv) fx_v
                          end v.
     Proof.
       destruct 1; eauto.
@@ -116,7 +121,7 @@ Section comp.
         forall v, computes_to c v -> P v.
 
       (* Relation to assist in building proofs of compuational_inv *)
-      Inductive CompInv : forall {A : Type}, Ensemble A -> @Comp names dom cod A -> Prop :=
+      Inductive CompInv : forall {A : Type}, Ensemble A -> Comp A -> Prop :=
       | Return_Inv : forall A (a : A) (P : Ensemble A),
                        P a -> CompInv P (Return a)
       | Bind_Inv : forall A B (PA : Ensemble A) (PB : Ensemble B) comp_a comp_f,
@@ -127,11 +132,11 @@ Section comp.
                      (forall a, P a -> P' a) -> CompInv P' (Pick P)
       | Call_Inv : forall f P P' comp_x,
                        @CompInv (dom f) P comp_x
-                       -> (forall x, P x -> CompInv P' (@lookup f x))
+                       -> (forall x, P x -> CompInv P' (@lookup _ f x))
                        -> CompInv P' (Call f comp_x).
 
       Lemma CompInv_inv A c (P : Ensemble A)
-      : CompInv P c -> match c in (@Comp _ _ _ A) return Ensemble A -> Prop with
+      : CompInv P c -> match c in (Comp A) return Ensemble A -> Prop with
                          | Return A x => fun P => P x
                          | Bind A B x f => fun PB => exists PA : Ensemble A,
                                                        CompInv PA x /\
@@ -139,7 +144,7 @@ Section comp.
                          | Pick A P => fun P' => (forall a, P a -> P' a)
                          | Call f x => fun P' => exists P,
                                                    CompInv P x
-                                                   /\ forall xv, P xv -> CompInv P' (@lookup f xv)
+                                                   /\ forall xv, P xv -> CompInv P' (@lookup _ f xv)
                        end P.
       Proof.
         destruct 1; eauto.
@@ -162,17 +167,15 @@ Section comp.
   End computes_to.
 
   Section is_computational.
-    Variable names : Type.
-    Variables dom cod : names -> Type.
-    Variable lookup : forall name, dom name -> @Comp names dom cod (cod name).
+    Context `{ctx : LookupContext}.
 
     (** A [Comp] is maximally computational if it could be written without [Pick].  For now, we don't permit [Call] in computational things, because the halting problem. *)
-    Inductive is_computational : forall A, @Comp names dom cod A -> Prop :=
+    Inductive is_computational : forall A, Comp A -> Prop :=
     | Return_is_computational : forall A (x : A), is_computational (Return x)
-    | Bind_is_computational : forall A B (cA : Comp _ _ A) (f : A -> Comp _ _ B),
+    | Bind_is_computational : forall A B (cA : Comp A) (f : A -> Comp B),
                                 is_computational cA
                                 -> (forall a,
-                                      @computes_to names dom cod lookup _ cA a -> is_computational (f a))
+                                      @computes_to _ _ cA a -> is_computational (f a))
                                 -> is_computational (Bind cA f)
 (*    | Call_is_computational : forall f x,
                                 is_computational x
@@ -181,12 +184,12 @@ Section comp.
                                       -> is_computational (@lookup f xv))
                                 -> is_computational (Call f x)*).
 
-    Theorem is_computational_inv A (c : @Comp names dom cod A)
+    Theorem is_computational_inv A (c : Comp A)
     : is_computational c
       -> match c with
            | Return _ _ => True
            | Bind _ _ x f => is_computational x
-                             /\ forall v, @computes_to names dom cod lookup _ x v
+                             /\ forall v, @computes_to _ _ x v
                                           -> is_computational (f v)
            | Pick _ _ => False
            | Call f x => False (*is_computational x
@@ -198,11 +201,11 @@ Section comp.
     Qed.
 
     (** It's possible to extract the value from a fully detiministic computation *)
-    Fixpoint is_computational_unique_val A (c : @Comp names dom cod A) {struct c}
-    : is_computational c -> { a | unique (computes_to lookup c) a }.
+    Fixpoint is_computational_unique_val A (c : Comp A) {struct c}
+    : is_computational c -> { a | unique (computes_to c) a }.
     Proof.
-      refine match c as c return is_computational c -> { a | unique (computes_to lookup c) a } with
-               | Return T x => fun _ => existT (unique (computes_to lookup (ret x)))
+      refine match c as c return is_computational c -> { a | unique (computes_to c) a } with
+               | Return T x => fun _ => existT (unique (computes_to (ret x)))
                                                x
                                                _
                | Pick _ _ => fun H => match is_computational_inv H with end
@@ -211,7 +214,7 @@ Section comp.
                     => let H' := is_computational_inv H in
                        let xv := @is_computational_unique_val _ _ (proj1 H') in
                        let fxv := @is_computational_unique_val _ _ (proj2 H' _ (proj1 (proj2_sig xv))) in
-                       exist (unique (computes_to _ _))
+                       exist (unique (computes_to _))
                              (proj1_sig fxv)
                              _
                | Call f x => fun H => match is_computational_inv H with end(*
@@ -239,15 +242,15 @@ Section comp.
                 ) ].
     Defined.
 
-    Definition is_computational_val A (c : @Comp names dom cod A) (H : is_computational c) : A
+    Definition is_computational_val A (c : Comp A) (H : is_computational c) : A
       := proj1_sig (@is_computational_unique_val A c H).
-    Definition is_computational_val_computes_to A (c : @Comp names dom cod A) (H : is_computational c) : computes_to lookup c (is_computational_val H)
+    Definition is_computational_val_computes_to A (c : Comp A) (H : is_computational c) : computes_to c (is_computational_val H)
       := proj1 (proj2_sig (@is_computational_unique_val A c H)).
-    Definition is_computational_val_unique A (c : @Comp names dom cod A) (H : is_computational c)
-    : forall x, computes_to lookup c x -> is_computational_val H = x
+    Definition is_computational_val_unique A (c : Comp A) (H : is_computational c)
+    : forall x, computes_to c x -> is_computational_val H = x
       := proj2 (proj2_sig (@is_computational_unique_val A c H)).
-    Definition is_computational_val_all_eq A (c : @Comp names dom cod A) (H : is_computational c)
-    : forall x y, computes_to lookup c x -> computes_to lookup c y -> x = y.
+    Definition is_computational_val_all_eq A (c : Comp A) (H : is_computational c)
+    : forall x y, computes_to c x -> computes_to c y -> x = y.
     Proof.
       intros.
       transitivity (@is_computational_val A c H); [ symmetry | ];
@@ -257,9 +260,7 @@ Section comp.
   End is_computational.
 
   Section monad.
-    Variable names : Type.
-    Variables dom cod : names -> Type.
-    Variable lookup : forall name, dom name -> @Comp names dom cod (cod name).
+    Context `{ctx : LookupContext}.
 
     Local Ltac t :=
       split;
@@ -275,30 +276,30 @@ Section comp.
                    | solve [ constructor ]
                    | eapply BindComputes; (eassumption || (try eassumption; [])) ].
 
-    Lemma bind_bind X Y Z (f : X -> @Comp names dom cod Y) (g : Y -> @Comp _ _ _ Z) x v
-    : computes_to lookup (Bind (Bind x f) g) v
-      <-> computes_to lookup (Bind x (fun u => Bind (f u) g)) v.
+    Lemma bind_bind X Y Z (f : X -> Comp Y) (g : Y -> Comp Z) x v
+    : computes_to (Bind (Bind x f) g) v
+      <-> computes_to (Bind x (fun u => Bind (f u) g)) v.
     Proof.
       t.
     Qed.
 
-    Lemma bind_unit X Y (f : X -> @Comp names dom cod Y) x v
-    : computes_to lookup (Bind (Return x) f) v
-      <-> computes_to lookup (f x) v.
+    Lemma bind_unit X Y (f : X -> Comp Y) x v
+    : computes_to (Bind (Return x) f) v
+      <-> computes_to (f x) v.
     Proof.
       t.
     Qed.
 
-    Lemma unit_bind X (x : @Comp names dom cod X) v
-    : computes_to lookup (Bind x (@Return _ _ _ X)) v
-      <-> computes_to lookup x v.
+    Lemma unit_bind X (x : Comp X) v
+    : computes_to (Bind x (@Return _ X)) v
+      <-> computes_to x v.
     Proof.
       t.
     Qed.
 
-    Lemma computes_under_bind X Y (f g : X -> @Comp names dom cod Y) x
-    : (forall x v, computes_to lookup (f x) v <-> computes_to lookup (g x) v) ->
-      (forall v, computes_to lookup (Bind x f) v <-> computes_to lookup (Bind x g) v).
+    Lemma computes_under_bind X Y (f g : X -> Comp Y) x
+    : (forall x v, computes_to (f x) v <-> computes_to (g x) v) ->
+      (forall v, computes_to (Bind x f) v <-> computes_to (Bind x g) v).
     Proof.
       t; split_iff; eauto.
     Qed.
@@ -308,26 +309,26 @@ Section comp.
   (** The old program might be non-deterministic, and the new program
       less so.  This means we want to say that if [new] can compute to
       [v], then [old] should be able to compute to [v], too. *)
-  Definition refine {A} {oldNames oldDom oldCod newNames newDom newCod}
-             oldLookup newLookup
-             (old : @Comp oldNames oldDom oldCod A)
-             (new : @Comp newNames newDom newCod A)
-    := forall v, computes_to newLookup new v -> computes_to oldLookup old v.
+  Definition refine {A}
+             {oldCtx newCtx : LookupContext}
+             (old : @Comp oldCtx A)
+             (new : @Comp newCtx A)
+    := forall v, computes_to new v -> computes_to old v.
   Definition refineBundled {A} (old new : BundledComp A)
-    := refine (Lookup old) (Lookup new) old new.
+    := refine old new.
 
   Global Arguments refineBundled : simpl never.
   Typeclasses Transparent refineBundled.
 
   (** Define a symmetrized version of [refine] for ease of rewriting *)
-  Definition refineEquiv {A} {oldNames oldDom oldCod newNames newDom newCod}
-             oldLookup newLookup
-             (old : @Comp oldNames oldDom oldCod A)
-             (new : @Comp newNames newDom newCod A)
-    := refine oldLookup newLookup old new /\ refine newLookup oldLookup new old.
+  Definition refineEquiv {A}
+             {oldCtx newCtx : LookupContext}
+             (old : @Comp oldCtx A)
+             (new : @Comp newCtx A)
+    := refine old new /\ refine new old.
 
   Definition refineBundledEquiv {A} (old new : BundledComp A)
-    := refineEquiv (Lookup old) (Lookup new) old new.
+    := refineEquiv old new.
 
   Global Arguments refineBundledEquiv : simpl never.
   Typeclasses Transparent refineBundledEquiv.
@@ -338,56 +339,50 @@ Section comp.
                                           | split
                                           | progress split_and ].
 
-  Global Program Instance refine_PreOrder A names dom cod lookup : PreOrder (@refine A names dom cod names dom cod lookup lookup).
+  Global Program Instance refine_PreOrder A `{LookupContext} : PreOrder (@refine A _ _).
   Global Program Instance refineBundled_PreOrder A : PreOrder (@refineBundled A).
-  Global Program Instance refineEquiv_Equivalence A names dom cod lookup : Equivalence (@refineEquiv A names dom cod names dom cod lookup lookup).
+  Global Program Instance refineEquiv_Equivalence A `{LookupContext} : Equivalence (@refineEquiv A _ _).
   Global Program Instance refineBundledEquiv_Equivalence A : Equivalence (@refineBundledEquiv A).
 
   Section monad_refine.
-    Variable names : Type.
-    Variables dom cod : names -> Type.
-    Variable lookup : forall name, dom name -> @Comp names dom cod (cod name).
+    Context `{ctx : LookupContext}.
 
-    Lemma refineEquiv_bind_bind X Y Z (f : X -> @Comp names dom cod Y) (g : Y -> @Comp _ _ _ Z) x
-    : refineEquiv lookup lookup
-                  (Bind (Bind x f) g)
+    Lemma refineEquiv_bind_bind X Y Z (f : X -> Comp Y) (g : Y -> Comp Z) x
+    : refineEquiv (Bind (Bind x f) g)
                   (Bind x (fun u => Bind (f u) g)).
     Proof.
       split; intro; apply bind_bind.
     Qed.
 
     Definition refineBundledEquiv_bind_bind
-    : forall X Y Z f g x, refineBundledEquiv ``[ _ with lookup ]`` ``[ _ with lookup ]``
+    : forall X Y Z f g x, refineBundledEquiv `[ _ ]` `[ _ ]`
       := refineEquiv_bind_bind.
 
-    Lemma refineEquiv_bind_unit X Y (f : X -> @Comp names dom cod Y) x
-    : refineEquiv lookup lookup
-                  (Bind (Return x) f)
+    Lemma refineEquiv_bind_unit X Y (f : X -> Comp Y) x
+    : refineEquiv (Bind (Return x) f)
                   (f x).
     Proof.
       split; intro; simpl; apply bind_unit.
     Qed.
 
     Definition refineBundledEquiv_bind_unit
-    : forall X Y f x, refineBundledEquiv ``[ _ with lookup ]`` ``[ _ with lookup ]``
+    : forall X Y f x, refineBundledEquiv `[ _ ]` `[ _ ]`
       := refineEquiv_bind_unit.
 
-    Lemma refineEquiv_unit_bind X (x : @Comp _ _ _ X)
-    : refineEquiv lookup lookup
-                  (Bind x (@Return _ _ _ X))
+    Lemma refineEquiv_unit_bind X (x : Comp X)
+    : refineEquiv (Bind x (@Return _ X))
                   x.
     Proof.
       split; intro; apply unit_bind.
     Qed.
 
     Definition refineBundledEquiv_unit_bind
-    : forall X x, refineBundledEquiv ``[ _ with lookup ]`` ``[ _ with lookup ]``
+    : forall X x, refineBundledEquiv `[ _ ]` `[ _ ]`
       := refineEquiv_unit_bind.
 
-    Lemma refineEquiv_under_bind X Y (f g : X -> @Comp _ _ _ Y) x
-          (eqv_f_g : forall x, refineEquiv lookup lookup (f x) (g x))
-    : refineEquiv lookup lookup
-                  (Bind x f)
+    Lemma refineEquiv_under_bind X Y (f g : X -> Comp Y) x
+          (eqv_f_g : forall x, refineEquiv (f x) (g x))
+    : refineEquiv (Bind x f)
                   (Bind x g).
     Proof.
       split; unfold refine; simpl in *; intros; eapply computes_under_bind;
@@ -396,8 +391,8 @@ Section comp.
 
     Definition refineBundledEquiv_under_bind
     : forall X Y f g x
-             (equv_f_g : forall x, refineBundledEquiv ``[ _ with lookup ]`` ``[ _ with lookup ]``),
-        refineBundledEquiv ``[ _ with lookup ]`` ``[ _ with lookup ]``
+             (equv_f_g : forall x, refineBundledEquiv `[ _ ]` `[ _ ]`),
+        refineBundledEquiv `[ _ ]` `[ _ ]`
       := refineEquiv_under_bind.
   End monad_refine.
 End comp.
@@ -407,8 +402,8 @@ Ltac inversion_by rule :=
                         | progress split_and
                         | apply_in_hyp_no_cbv_match rule ].
 
-Add Parametric Relation A names dom cod lookup
-: (@Comp names dom cod A) (@refine A names dom cod names dom cod lookup lookup)
+Add Parametric Relation A `{LookupContext}
+: (Comp A) (@refine A _ _)
   reflexivity proved by reflexivity
   transitivity proved by transitivity
     as refine_rel.
@@ -419,8 +414,8 @@ Add Parametric Relation A
   transitivity proved by transitivity
     as refineBundled_rel.
 
-Add Parametric Relation A names dom cod lookup
-: (@Comp names dom cod A) (@refineEquiv A names dom cod names dom cod lookup lookup)
+Add Parametric Relation A `{LookupContext}
+: (Comp A) (@refineEquiv A _ _)
   reflexivity proved by reflexivity
   symmetry proved by symmetry
   transitivity proved by transitivity
@@ -435,10 +430,10 @@ Add Parametric Relation A
 
 Local Ltac t := unfold impl; intros; repeat (eapply_hyp || etransitivity).
 
-Add Parametric Morphism A names dom cod lookup
-: (@refine A names dom cod names dom cod lookup lookup)
+Add Parametric Morphism A `{LookupContext}
+: (@refine A _ _)
   with signature
-  (@refine A names dom cod names dom cod lookup lookup) --> (@refine A names dom cod names dom cod lookup lookup) ++> impl
+  (@refine A _ _) --> (@refine A _ _) ++> impl
     as refine_refine.
 Proof. t. Qed.
 
@@ -466,12 +461,12 @@ Proof. t. Qed.*)
 
 Hint Constructors CompInv computes_to.
 
-Add Parametric Morphism names dom cod lookup A B
-: (@Bind names dom cod A B)
+Add Parametric Morphism `{LookupContext} A B
+: (@Bind _ A B)
     with signature
-    (@refine A names dom cod names dom cod lookup lookup)
-      ==> (pointwise_relation _ (@refine B names dom cod names dom cod lookup lookup))
-      ==> (@refine B names dom cod names dom cod lookup lookup)
+    (@refine A _ _)
+      ==> (pointwise_relation _ (@refine B _ _))
+      ==> (@refine B _ _)
       as refine_bind.
 Proof.
   simpl; intros.
@@ -481,12 +476,12 @@ Proof.
   eauto.
 Qed.
 
-Add Parametric Morphism names dom cod lookup A B
-: (@Bind names dom cod A B)
+Add Parametric Morphism `{LookupContext} A B
+: (@Bind _ A B)
     with signature
-    (@refineEquiv A names dom cod names dom cod lookup lookup)
-      ==> (pointwise_relation _ (@refineEquiv B names dom cod names dom cod lookup lookup))
-      ==> (@refineEquiv B names dom cod names dom cod lookup lookup)
+    (@refineEquiv A _ _)
+      ==> (pointwise_relation _ (@refineEquiv B _ _))
+      ==> (@refineEquiv B _ _)
       as refineEquiv_bind.
 Proof.
   simpl; intros.
@@ -497,7 +492,7 @@ Proof.
   eauto.
 Qed.
 
-(*Add Parametric Morphism names dom cod lookup A B
+(*Add Parametric Morphism `{LookupContext} A B
 : (@Bind names dom cod A B)
     with signature
     (@refineEquiv A names dom cod names dom cod lookup lookup)
@@ -514,190 +509,239 @@ Proof.
 Qed.*)
 
 Local Arguments impl _ _ / .
-Global Arguments computational_inv [names dom cod] lookup [A] P c / .
+Global Arguments computational_inv {_} [A] P c / .
 
-Add Parametric Morphism names dom cod lookup A P : (@computational_inv names dom cod lookup A P)
+Add Parametric Morphism `{LookupContext} A P : (@computational_inv _ A P)
   with signature
-  (@refine A names dom cod names dom cod lookup lookup) ++> impl
+  (@refine A _ _) ++> impl
     as refineCompInv.
 Proof. simpl; eauto. Qed.
 
-Section general_refine_lemmas.
-  Local Ltac t :=
-    repeat first [ progress eauto
-                 | eassumption
-                 | progress split_iff
-                 | progress inversion_by computes_to_inv
-                 | progress subst
-                 | intro
-                 | econstructor
-                 | erewrite is_computational_val_unique
-                 | progress destruct_head_hnf prod
-                 | progress destruct_head_hnf and
-                 | progress specialize_all_ways ].
 
-  Lemma refineEquiv_is_computational A {names dom cod names' dom' cod'} (c : @Comp names dom cod A) lookup lookup' (CompC : is_computational lookup c)
-  : @refineEquiv _ names dom cod names' dom' cod' lookup lookup'
+Local Ltac t_refine :=
+  repeat first [ progress simpl in *
+               | progress eauto
+               | eassumption
+               | reflexivity
+               | progress split_iff
+               | progress inversion_by computes_to_inv
+               | progress subst
+               | intro
+               | econstructor
+               | erewrite is_computational_val_unique
+               | progress destruct_head_hnf prod
+               | progress destruct_head_hnf and
+               | progress specialize_all_ways ].
+
+Section structural.
+  Inductive refineBundled_structural {ctx1 ctx2 : LookupContext}
+  : forall A, @Comp ctx1 A -> @Comp ctx2 A -> Prop :=
+| rbEq_Return : forall A (x : A), refineBundled_structural (Return x) (Return x)
+| rbEq_Bind : forall A B c1 c2 f1 f2,
+                refineBundled_structural c1 c2
+                -> (forall v : A,
+                      @computes_to ctx1 _ c1 v
+                      -> @computes_to ctx2 _ c2 v
+                      -> refineBundled_structural (f1 v) (f2 v))
+                -> @refineBundled_structural _ _ B (Bind c1 f1) (Bind c2 f2)
+| rbEq_Pick : forall A P, @refineBundled_structural ctx1 ctx2 A (Pick P) (Pick P).
+
+
+  Lemma refineBundled_structural_impl_refineBundledEquiv {A} (c1 c2 : BundledComp A)
+  : refineBundled_structural c1 c2 -> refineBundledEquiv c1 c2.
+  Proof.
+    destruct c1 as [ctx1 c1], c2 as [ctx2 c2]; simpl.
+    induction 1; t_refine.
+  Qed.
+End structural.
+
+Ltac refineBundledEquiv_reflexivity_ignore_context :=
+  apply refineBundled_structural_impl_refineBundledEquiv;
+  simpl;
+  repeat (econstructor || intro).
+
+Ltac equate_evar_context :=
+  unfold refineBundledEquiv, refineBundled; simpl;
+  lazymatch goal with
+    | [ |- @refineEquiv ?A ?ctx1 (@CompContext ?B ?e) ?v1 ?v2 ]
+      => is_evar e; refine (_ : @refineEquiv A ctx1 (@CompContext B {| CompContext := ctx1 |}) v1 v2)
+    | [ |- @refine ?A ?ctx1 (@CompContext ?B ?e) ?v1 ?v2 ]
+      => is_evar e; refine (_ : @refine A ctx1 (@CompContext B {| CompContext := ctx1 |}) v1 v2)
+  end;
+  simpl.
+
+Ltac etransitivity_context :=
+  etransitivity;
+  [ equate_evar_context | refineBundledEquiv_reflexivity_ignore_context ].
+
+Section general_refine_lemmas.
+  Lemma refineEquiv_is_computational {A} {ctx1 ctx2 : LookupContext} {c} (CompC : @is_computational ctx1 A c)
+  : @refineEquiv _ ctx1 ctx2
                 c (ret (is_computational_val CompC)).
   Proof.
     unfold refineEquiv, refine.
     pose proof (is_computational_val_computes_to CompC).
-    t.
+    t_refine.
   Qed.
 
-  Definition refineBundledEquiv_is_computational A {names dom cod} (c : BundledComp A) lookup
-  : forall (CompC : is_computational (Lookup c) c),
-      refineBundledEquiv c (@Bundle A names dom cod (ret (is_computational_val CompC)) lookup)
-    := refineEquiv_is_computational lookup.
+  Definition refineBundledEquiv_is_computational A {ctx1 : LookupContext} (c : BundledComp A)
+  : forall (CompC : is_computational c),
+      refineBundledEquiv c ``[ ret (is_computational_val CompC) with ctx1 ]``
+    := @refineEquiv_is_computational A _ ctx1 c.
 
-  Lemma refine_pick A {names dom cod names' dom' cod'} lookup lookup'
-        (P : A -> Prop) c (H : forall x, computes_to lookup' c x -> P x)
-  : @refine A names dom cod names' dom' cod' lookup lookup'
+  Lemma refine_pick A {ctx1 ctx2 : LookupContext}
+        (P : A -> Prop) c (H : forall x, computes_to c x -> P x)
+  : @refine A ctx1 ctx2
             { x : A | P x }%comp
             c.
-  Proof. t. Qed.
+  Proof. t_refine. Qed.
 
-  Definition refineBundled_pick A {names dom cod} lookup
+  Definition refineBundled_pick A {ctx1 : LookupContext}
              P (c : BundledComp A)
-  : _ -> refineBundled ``[ { x : A | P x }%comp with lookup ]``
+  : _ -> refineBundled ``[ { x : A | P x }%comp with ctx1 ]``
                        c
-    := @refine_pick _ names dom cod _ _ _ lookup _ P c.
+    := @refine_pick _ _ _ P c.
 
-  Lemma refine_pick_pick A {names dom cod names' dom' cod'} lookup lookup' (P1 P2 : A -> Prop)
+  Lemma refine_pick_pick A {ctx1 ctx2 : LookupContext} (P1 P2 : A -> Prop)
         (H : forall x, P2 x -> P1 x)
-  : @refine _ names dom cod names' dom' cod' lookup lookup'
+  : @refine _ ctx1 ctx2
             { x : A | P1 x }%comp
             { x : A | P2 x }%comp.
-  Proof. t. Qed.
+  Proof. t_refine. Qed.
 
   Definition refineBundled_pick_pick
-  : forall A {names dom cod names' dom' cod'} lookup lookup' P1 P2 H,
-      refineBundled ``[ _ with lookup ]``
-                    ``[ _ with lookup' ]``
+  : forall A {ctx1 ctx2} P1 P2 H,
+      refineBundled ``[ _ with ctx1 ]``
+                    ``[ _ with ctx2 ]``
     := refine_pick_pick.
 
-  Lemma refineEquiv_pick_pick A {names dom cod names' dom' cod'} lookup lookup' (P1 P2 : A -> Prop)
+  Lemma refineEquiv_pick_pick A {ctx1 ctx2} (P1 P2 : A -> Prop)
         (H : forall x, P1 x <-> P2 x)
-  : @refineEquiv _ names dom cod names' dom' cod' lookup lookup'
+  : @refineEquiv _ ctx1 ctx2
                  { x : A | P1 x }%comp
                  { x : A | P2 x }%comp.
-  Proof. t. Qed.
+  Proof. t_refine. Qed.
 
   Definition refineBundledEquiv_pick_pick
-  : forall A {names dom cod names' dom' cod'} lookup lookup' P1 P2 H,
-      refineBundledEquiv ``[ _ with lookup ]``
-                         ``[ _ with lookup' ]``
+  : forall A {ctx1 ctx2} P1 P2 H,
+      refineBundledEquiv ``[ _ with ctx1 ]``
+                         ``[ _ with ctx2 ]``
     := refineEquiv_pick_pick.
 
-  Lemma refineEquiv_pick_pair {names dom cod names' dom' cod'} lookup lookup' A B (PA : A -> Prop) (PB : B -> Prop)
-  : @refineEquiv _ names dom cod names' dom' cod' lookup lookup'
+  Lemma refineEquiv_pick_pair {ctx1 ctx2} A B (PA : A -> Prop) (PB : B -> Prop)
+  : @refineEquiv _ ctx1 ctx2
                  { x : A * B | PA (fst x) /\ PB (snd x) }%comp
                  (a <- { a : A | PA a };
                   b <- { b : B | PB b };
                   ret (a, b))%comp.
-  Proof. t. Qed.
+  Proof. t_refine. Qed.
 
   Definition refineEquivBundled_pick_pair
-  : forall A {names dom cod names' dom' cod'} lookup lookup' P1 P2 H,
-      refineBundledEquiv ``[ _ with lookup ]``
-                         ``[ _ with lookup' ]``
+  : forall A {ctx1 ctx2} P1 P2 H,
+      refineBundledEquiv ``[ _ with ctx1 ]``
+                         ``[ _ with ctx2 ]``
     := refineEquiv_pick_pick.
 
-  Definition refineEquiv_split_ex {names dom cod names' dom' cod'} lookup lookup' A B (P : A -> Prop) (P' : A -> B -> Prop)
-  : @refineEquiv _ names dom cod names' dom' cod' lookup lookup'
+  Definition refineEquiv_split_ex {ctx1 ctx2} A B (P : A -> Prop) (P' : A -> B -> Prop)
+  : @refineEquiv _ ctx1 ctx2
                  { b | exists a, P a /\ P' a b }%comp
                  (a <- { a | P a /\ exists b, P' a b };
                   { b | P' a b })%comp.
-  Proof. t. Qed.
+  Proof. t_refine. Qed.
 
   Definition refineBundledEquiv_split_ex
-  : forall {names dom cod names' dom' cod'} lookup lookup' A B P P',
+  : forall {ctx1 ctx2} A B P P',
       refineBundledEquiv `[ _ ]` `[ _ ]`
     := @refineEquiv_split_ex.
 
-  Definition refineEquiv_pick_contr_ret {names dom cod names' dom' cod'} lookup lookup' A (P : A -> Prop)
+  Definition refineEquiv_pick_contr_ret {ctx1 ctx2} A (P : A -> Prop)
              (x : A) (H : unique P x)
-  : @refineEquiv _ names dom cod names' dom' cod' lookup lookup'
+  : @refineEquiv _ ctx1 ctx2
                  { y | P y }
                  (ret x).
-  Proof. t. Qed.
+  Proof. t_refine. Qed.
 
-  Definition refineEquiv_pick_eq {names dom cod names' dom' cod'} lookup lookup'
+  Definition refineEquiv_pick_eq {ctx1 ctx2}
              A (x : A)
-  : @refineEquiv _ names dom cod names' dom' cod' lookup lookup'
+  : @refineEquiv _ ctx1 ctx2
                  { y | y = x }%comp
                  (ret x).
-  Proof. t. Qed.
+  Proof. t_refine. Qed.
 
   Definition refineBundledEquiv_pick_eq
-  : forall {names dom cod names' dom' cod'} lookup lookup'
+  : forall {ctx1 ctx2}
            A (x : A),
       refineBundledEquiv `[ _ ]` `[ _ ]`
     := @refineEquiv_pick_eq.
 
-  Definition refineEquiv_pick_eq' {names dom cod names' dom' cod'} lookup lookup'
+  Definition refineEquiv_pick_eq' {ctx1 ctx2}
              A (x : A)
-  : @refineEquiv _ names dom cod names' dom' cod' lookup lookup'
+  : @refineEquiv _ ctx1 ctx2
                  { y | x = y }%comp
                  (ret x).
-  Proof. t. Qed.
+  Proof. t_refine. Qed.
 
   Definition refineBundledEquiv_pick_eq'
-  : forall {names dom cod names' dom' cod'} lookup lookup'
+  : forall {ctx1 ctx2}
            A (x : A),
       refineBundledEquiv `[ _ ]` `[ _ ]`
     := @refineEquiv_pick_eq'.
 
-  Definition refineBundledEquiv_split_func_ex {names dom cod names' dom' cod'} lookup lookup'
+  Definition refineBundledEquiv_split_func_ex {ctx1 ctx2}
              A B (P : A -> Prop) (f : A -> B)
-  : refineBundledEquiv (@Bundle _ names dom cod { b | exists a, P a /\ b = f a}%comp lookup)
-                       (@Bundle _ names' dom' cod'
-                                (a <- { a | P a};
-                                 ret (f a))%comp
-                                lookup').
+  : refineBundledEquiv ``[ { b | exists a, P a /\ b = f a}%comp with ctx1 ]``
+                       ``[ (a <- { a | P a};
+                            ret (f a))%comp
+                           with ctx2 ]``.
   Proof.
     repeat setoid_rewrite refineBundledEquiv_split_ex.
-    (** I want to just [setoid_rewrite refineBundledEquiv_pick_eq].  But I can't because things don't line up nicely, and there are no parameterized setoid relations.  :-( *)
-    setoid_rewrite refineBundledEquiv_pick_eq.
-    erewrite refineEquiv_pick_pick.
-    - reflexivity.
-    - abstract (repeat (intro || esplit); intuition).
-  Qed.
-
-  Definition refineEquiv_split_func_ex {names dom cod names' dom' cod'} lookup lookup'
-             A B (P : A -> Prop) (f : A -> B)
-  : @refineEquiv _ names dom cod names' dom' cod' lookup lookup'
-                 { b | exists a, P a /\ b = f a}%comp
-                 (a <- { a | P a};
-                  ret (f a))%comp.
-  Proof.
-    repeat setoid_rewrite refineBundledEquiv_split_ex.
+    (** I want to just [setoid_rewrite refineBundledEquiv_pick_eq].  But I can't because things don't line up nicely, and there are no parameterized setoid relations.  :-(  So instead we need to [etransitivity_context] instead. *)
+    etransitivity_context.
     setoid_rewrite refineEquiv_pick_eq.
-    erewrite refineEquiv_pick_pick.
+    (** [erewrite] is buggy: https://coq.inria.fr/bugs/show_bug.cgi?id=3244 *)
+    erewrite (@refineEquiv_pick_pick _ _ _).
     - reflexivity.
     - abstract (repeat (intro || esplit); intuition).
   Qed.
 
-  Definition refineEquiv_split_func_ex2 A A' B (P : A -> Prop) (P' : A' -> Prop)
+  Definition refineEquiv_split_func_ex {ctx1 ctx2}
+  : forall A B (P : A -> Prop) (f : A -> B),
+      @refineEquiv _ ctx1 ctx2
+                   { b | exists a, P a /\ b = f a}%comp
+                   (a <- { a | P a};
+                    ret (f a))%comp
+    := refineBundledEquiv_split_func_ex.
+
+  Definition refineBundledEquiv_split_func_ex2 {ctx1 ctx2} A A' B (P : A -> Prop) (P' : A' -> Prop)
              (f : A -> A' -> B)
-  : refineEquiv { b | exists a, P a /\ exists a', P' a' /\ b = f a a'}%comp
-                (a <- { a | P a};
-                 a' <- { a' | P' a'};
-                 ret (f a a'))%comp.
+  : refineBundledEquiv ``[ { b | exists a, P a /\ exists a', P' a' /\ b = f a a'} with ctx1 ]``
+                       ``[ (a <- { a | P a};
+                            a' <- { a' | P' a'};
+                            ret (f a a'))
+                           with ctx2 ]``.
   Proof.
-    repeat setoid_rewrite refineEquiv_split_ex.
-    setoid_rewrite refineEquiv_pick_eq.
+    etransitivity_context.
+    (** >:-(   We shouldn't need to clear the context to get typeclass resolution and setoid rewriting to work. *)
+    clear.
+    repeat setoid_rewrite (@refineEquiv_split_ex _ _).
+    setoid_rewrite (@refineEquiv_pick_eq _ _).
     split; intro; intros;
     inversion_by computes_to_inv; subst;
     repeat econstructor; eassumption.
   Qed.
+
+  Definition refineEquiv_split_func_ex2 {ctx1 ctx2}
+  : forall A A' B (P : A -> Prop) (P' : A' -> Prop)
+           (f : A -> A' -> B),
+      refineEquiv _ _
+    := @refineBundledEquiv_split_func_ex2 ctx1 ctx2.
 End general_refine_lemmas.
 
 Create HintDb refine_monad discriminated.
 
 (*Hint Rewrite refine_bind_bind refine_bind_unit refine_unit_bind : refine_monad.
 Hint Rewrite <- refine_bind_bind' refine_bind_unit' refine_unit_bind' : refine_monad.*)
-Hint Rewrite refineEquiv_bind_bind refineEquiv_bind_unit refineEquiv_unit_bind : refine_monad.
+Hint Rewrite @refineEquiv_bind_bind @refineEquiv_bind_unit @refineEquiv_unit_bind : refine_monad.
 (* Ideally we would throw refineEquiv_under_bind in here as well, but it gets stuck *)
 
 
